recursion done in the wrong direction...

Low/ScalarMult_gen_small.v
@@ -1,60 +1,4 @@
-(*
-int crypto_scalarmult(u8 *q,const u8 *n,const u8 *p)
-{
-  u8 z[32];
-  i64 x[80],r;
-  int i;
-  gf a,b,c,d,e,f;
-  FOR(i,31) z[i]=n[i];
-  z[31]=(n[31]&127)|64;
-  z[0]&=248;
-  unpack25519(x,p);
-  FOR(i,16) {
-    b[i]=x[i];
-    d[i]=a[i]=c[i]=0;
-  }
-  a[0]=d[0]=1;
-  for(i=254;i>=0;--i) {
-    r=(z[i>>3]>>(i&7))&1;
-    sel25519(a,b,r);
-    sel25519(c,d,r);
-    A(e,a,c);
-    Z(a,a,c);
-    A(c,b,d);
-    Z(b,b,d);
-    S(d,e);
-    S(f,a);
-    M(a,c,a);
-    M(c,b,e);
-    A(e,a,c);
-    Z(a,a,c);
-    S(b,a);
-    Z(c,d,f);
-    M(a,c,_121665);
-    A(a,a,d);
-    M(c,c,a);
-    M(a,d,f);
-    M(d,b,x);
-    S(b,e);
-    sel25519(a,b,r);
-    sel25519(c,d,r);
-  }
-  FOR(i,16) {
-    x[i+16]=a[i];
-    x[i+32]=c[i];
-    x[i+48]=b[i];
-    x[i+64]=d[i];
-  }
-  inv25519(x+32,x+32);
-  M(x+16,x+16,x+32);
-  pack25519(q,x+16);
-  return 0;
-}
-*)
-
 Require Import Tweetnacl.Libs.Export.
-Require Import Tweetnacl.Low.ScalarMult_gen_small.
-Require Import Tweetnacl.Low.Get_abcdef.
 
 Section ScalarRec.
 
@@ -66,88 +10,73 @@ Variable _121665: list Z.
 Variable Sel25519 : Z -> list Z -> list Z -> list Z.
 Variable getbit : Z -> list Z -> Z.
 
-Fixpoint montgomery_rec_gen (m : nat) (z a b c d e f x : list Z) : (list Z * list Z * list Z * list Z * list Z * list Z) :=
-  match m with
-  | 0%nat => (a,b,c,d,e,f)
-  | S n => 
-      let r := getbit (Z.of_nat n) z in
-      let (a, b) := (Sel25519 r a b, Sel25519 r b a) in
-      let (c, d) := (Sel25519 r c d, Sel25519 r d c) in
-      let e := A a c in
-      let a := Zub a c in
-      let c := A b d in
-      let b := Zub b d in
-      let d := Sq e in
-      let f := Sq a in
-      let a := M c a in
-      let c := M b e in
-      let e := A a c in
-      let a := Zub a c in
-      let b := Sq a in
-      let c := Zub d f in
-      let a := M c _121665 in
-      let a := A a d in
-      let c := M c a in
-      let a := M d f in
-      let d := M b x in
-      let b := Sq e in
-      let (a, b) := (Sel25519 r a b, Sel25519 r b a) in
-      let (c, d) := (Sel25519 r c d, Sel25519 r d c) in
-      montgomery_rec_gen n z a b c d e f x
-    end.
+Definition fa r (a b c d e f x:list Z) :=
+  Sel25519 r
+     (M (Sq (A (Sel25519 r a b) (Sel25519 r c d)))
+        (Sq (Zub (Sel25519 r a b) (Sel25519 r c d))))
+     (Sq
+        (A
+           (M (A (Sel25519 r b a) (Sel25519 r d c))
+              (Zub (Sel25519 r a b) (Sel25519 r c d)))
+           (M (Zub (Sel25519 r b a) (Sel25519 r d c))
+              (A (Sel25519 r a b) (Sel25519 r c d))))).
 
-Definition montgomery_step_gen (m:nat) (z a b c d e f x : list Z) : (list Z * list Z * list Z * list Z * list Z * list Z)  :=
-      let r := getbit (Z.of_nat m) z in
-      let (a, b) := (Sel25519 r a b, Sel25519 r b a) in
-      let (c, d) := (Sel25519 r c d, Sel25519 r d c) in
-      let e := A a c in
-      let a := Zub a c in
-      let c := A b d in
-      let b := Zub b d in
-      let d := Sq e in
-      let f := Sq a in
-      let a := M c a in
-      let c := M b e in
-      let e := A a c in
-      let a := Zub a c in
-      let b := Sq a in
-      let c := Zub d f in
-      let a := M c _121665 in
-      let a := A a d in
-      let c := M c a in
-      let a := M d f in
-      let d := M b x in
-      let b := Sq e in
-      let (a, b) := (Sel25519 r a b, Sel25519 r b a) in
-      let (c, d) := (Sel25519 r c d, Sel25519 r d c) in
-      (a,b,c,d,e,f).
-(*     end. *)
+Definition fb r (a b c d e f x:list Z) :=
+  Sel25519 r
+     (Sq
+        (A
+           (M (A (Sel25519 r b a) (Sel25519 r d c))
+              (Zub (Sel25519 r a b) (Sel25519 r c d)))
+           (M (Zub (Sel25519 r b a) (Sel25519 r d c))
+              (A (Sel25519 r a b) (Sel25519 r c d)))))
+     (M (Sq (A (Sel25519 r a b) (Sel25519 r c d)))
+        (Sq (Zub (Sel25519 r a b) (Sel25519 r c d)))).
 
+Definition fc r (a b c d e f x:list Z) :=
+Sel25519 r
+  (M
+     (Zub (Sq (A (Sel25519 r a b) (Sel25519 r c d)))
+        (Sq (Zub (Sel25519 r a b) (Sel25519 r c d))))
+     (A
+        (M
+           (Zub (Sq (A (Sel25519 r a b) (Sel25519 r c d)))
+              (Sq (Zub (Sel25519 r a b) (Sel25519 r c d)))) _121665)
+        (Sq (A (Sel25519 r a b) (Sel25519 r c d)))))
+  (M
+     (Sq
+        (Zub
+           (M (A (Sel25519 r b a) (Sel25519 r d c))
+              (Zub (Sel25519 r a b) (Sel25519 r c d)))
+           (M (Zub (Sel25519 r b a) (Sel25519 r d c))
+              (A (Sel25519 r a b) (Sel25519 r c d))))) x).
 
-Lemma opt_montgomery_rec_step_gen : forall n z a b c d e f x,
-  montgomery_rec_gen (S n) z a b c d e f x = 
-  montgomery_rec_gen n z 
-  (get_a (montgomery_step_gen n z a b c d e f x))
-  (get_b (montgomery_step_gen n z a b c d e f x))
-  (get_c (montgomery_step_gen n z a b c d e f x))
-  (get_d (montgomery_step_gen n z a b c d e f x))
-  (get_e (montgomery_step_gen n z a b c d e f x))
-  (get_f (montgomery_step_gen n z a b c d e f x))
-  x.
-Proof. reflexivity. Qed.
+Definition fd r (a b c d e f x:list Z) :=
+Sel25519 r
+  (M
+     (Sq
+        (Zub
+           (M (A (Sel25519 r b a) (Sel25519 r d c))
+              (Zub (Sel25519 r a b) (Sel25519 r c d)))
+           (M (Zub (Sel25519 r b a) (Sel25519 r d c))
+              (A (Sel25519 r a b) (Sel25519 r c d))))) x)
+  (M
+     (Zub (Sq (A (Sel25519 r a b) (Sel25519 r c d)))
+        (Sq (Zub (Sel25519 r a b) (Sel25519 r c d))))
+     (A
+        (M
+           (Zub (Sq (A (Sel25519 r a b) (Sel25519 r c d)))
+              (Sq (Zub (Sel25519 r a b) (Sel25519 r c d)))) _121665)
+        (Sq (A (Sel25519 r a b) (Sel25519 r c d))))).
 
-Lemma opt_montgomery_rec_step_gen_ext : forall n z a b c d e f e' f' x,
-  montgomery_rec_gen (S n) z a b c d e' f' x = 
-  montgomery_rec_gen n z 
-  (get_a (montgomery_step_gen n z a b c d e f x))
-  (get_b (montgomery_step_gen n z a b c d e f x))
-  (get_c (montgomery_step_gen n z a b c d e f x))
-  (get_d (montgomery_step_gen n z a b c d e f x))
-  (get_e (montgomery_step_gen n z a b c d e f x))
-  (get_f (montgomery_step_gen n z a b c d e f x))
-  x.
-Proof. reflexivity. Qed.
+Definition fe r (a b c d e f x:list Z) :=
+A
+  (M (A (Sel25519 r b a) (Sel25519 r d c))
+     (Zub (Sel25519 r a b) (Sel25519 r c d)))
+  (M (Zub (Sel25519 r b a) (Sel25519 r d c))
+     (A (Sel25519 r a b) (Sel25519 r c d))).
 
+Definition ff r (a b c d e f x:list Z) :=
+  Sq (Zub (Sel25519 r a b) (Sel25519 r c d)).
 
 Close Scope Z.
 
@@ -169,10 +98,8 @@ Variable _121665_Zlength : Zlength _121665 = 16.
 
 Close Scope Z.
 
-Local Ltac solve_montgomery_step_gen_length :=
+Local Ltac solve_small_montgomery_step_gen_length :=
   intros;
-  rewrite /montgomery_step_gen;
-  rewrite /get_a /get_b /get_c /get_d /get_e /get_f;
   rewrite /fa /fb /fc /fd /fe /ff;
   repeat match goal with
     | _ => orewrite Sel25519_length
@@ -182,80 +109,42 @@ Local Ltac solve_montgomery_step_gen_length :=
     | _ => orewrite Zub_length
   end ; reflexivity.
 
-Lemma get_a_montgomery_step_gen_length : forall z a b c d e f x n,
+Lemma fa_length : forall r a b c d e f x,
   length a = 16 -> length b = 16 -> length c = 16 ->
   length d = 16 -> length e = 16 -> length f = 16 -> length x = 16 ->
-  length (get_a (montgomery_step_gen n z a b c d e f x)) = 16.
-Proof. solve_montgomery_step_gen_length. Qed.
-Lemma get_b_montgomery_step_gen_length : forall z a b c d e f x n,
+  length (fa r a b c d e f x) = 16.
+Proof. solve_small_montgomery_step_gen_length. Qed.
+Lemma fb_length : forall r a b c d e f x,
   length a = 16 -> length b = 16 -> length c = 16 ->
   length d = 16 -> length e = 16 -> length f = 16 -> length x = 16 ->
-  length (get_b (montgomery_step_gen n z a b c d e f x)) = 16.
-Proof. solve_montgomery_step_gen_length. Qed.
-Lemma get_c_montgomery_step_gen_length : forall z a b c d e f x n,
+  length (fb r a b c d e f x) = 16.
+Proof. solve_small_montgomery_step_gen_length. Qed.
+Lemma fc_length : forall r a b c d e f x,
   length a = 16 -> length b = 16 -> length c = 16 ->
   length d = 16 -> length e = 16 -> length f = 16 -> length x = 16 ->
-  length (get_c (montgomery_step_gen n z a b c d e f x)) = 16.
-Proof. solve_montgomery_step_gen_length. Qed.
-Lemma get_d_montgomery_step_gen_length : forall z a b c d e f x n,
+  length (fc r a b c d e f x) = 16.
+Proof. solve_small_montgomery_step_gen_length. Qed.
+Lemma fd_length : forall r a b c d e f x,
   length a = 16 -> length b = 16 -> length c = 16 ->
   length d = 16 -> length e = 16 -> length f = 16 -> length x = 16 ->
-  length (get_d (montgomery_step_gen n z a b c d e f x)) = 16.
-Proof. solve_montgomery_step_gen_length. Qed.
-Lemma get_e_montgomery_step_gen_length : forall z a b c d e f x n,
+  length (fd r a b c d e f x) = 16.
+Proof. solve_small_montgomery_step_gen_length. Qed.
+Lemma fe_length : forall r a b c d e f x,
   length a = 16 -> length b = 16 -> length c = 16 ->
   length d = 16 -> length e = 16 -> length f = 16 -> length x = 16 ->
-  length (get_e (montgomery_step_gen n z a b c d e f x)) = 16.
-Proof. solve_montgomery_step_gen_length. Qed.
-Lemma get_f_montgomery_step_gen_length : forall z a b c d e f x n,
+  length (fe r a b c d e f x) = 16.
+Proof. solve_small_montgomery_step_gen_length. Qed.
+Lemma ff_length : forall r a b c d e f x,
   length a = 16 -> length b = 16 -> length c = 16 ->
   length d = 16 -> length e = 16 -> length f = 16 -> length x = 16 ->
-  length (get_f (montgomery_step_gen n z a b c d e f x)) = 16.
-Proof. solve_montgomery_step_gen_length. Qed.
-
-Lemma get_a_montgomery_rec_gen_length : forall n z a b c d e f x,
-  length a = 16 -> length b = 16 -> length c = 16 ->
-  length d = 16 -> length e = 16 -> length f = 16 -> length x = 16 ->
-  length (get_a (montgomery_rec_gen n z a b c d e f x)) = 16.
-Proof. induction n; intros ; [assumption|] ; simpl.
-apply IHn ; try assumption ; solve_montgomery_step_gen_length. Qed.
-Lemma get_b_montgomery_rec_gen_length : forall n z a b c d e f x,
-  length a = 16 -> length b = 16 -> length c = 16 ->
-  length d = 16 -> length e = 16 -> length f = 16 -> length x = 16 ->
-  length (get_b (montgomery_rec_gen n z a b c d e f x)) = 16.
-Proof. induction n; intros ; [assumption|] ; simpl.
-apply IHn ; try assumption ; solve_montgomery_step_gen_length. Qed.
-Lemma get_c_montgomery_rec_gen_length : forall n z a b c d e f x,
-  length a = 16 -> length b = 16 -> length c = 16 ->
-  length d = 16 -> length e = 16 -> length f = 16 -> length x = 16 ->
-  length (get_c (montgomery_rec_gen n z a b c d e f x)) = 16.
-Proof. induction n; intros ; [assumption|] ; simpl.
-apply IHn ; try assumption ; solve_montgomery_step_gen_length. Qed.
-Lemma get_d_montgomery_rec_gen_length : forall n z a b c d e f x,
-  length a = 16 -> length b = 16 -> length c = 16 ->
-  length d = 16 -> length e = 16 -> length f = 16 -> length x = 16 ->
-  length (get_d (montgomery_rec_gen n z a b c d e f x)) = 16.
-Proof. induction n; intros ; [assumption|] ; simpl.
-apply IHn ; try assumption ; solve_montgomery_step_gen_length. Qed.
-Lemma get_e_montgomery_rec_gen_length : forall n z a b c d e f x,
-  length a = 16 -> length b = 16 -> length c = 16 ->
-  length d = 16 -> length e = 16 -> length f = 16 -> length x = 16 ->
-  length (get_e (montgomery_rec_gen n z a b c d e f x)) = 16.
-Proof. induction n; intros ; [assumption|] ; simpl.
-apply IHn ; try assumption ; solve_montgomery_step_gen_length. Qed.
-Lemma get_f_montgomery_rec_gen_length : forall n z a b c d e f x,
-  length a = 16 -> length b = 16 -> length c = 16 ->
-  length d = 16 -> length e = 16 -> length f = 16 -> length x = 16 ->
-  length (get_f (montgomery_rec_gen n z a b c d e f x)) = 16.
-Proof. induction n; intros ; [assumption|] ; simpl.
-apply IHn ; try assumption ; solve_montgomery_step_gen_length. Qed.
+  length (ff r a b c d e f x) = 16.
+Proof. solve_small_montgomery_step_gen_length. Qed.
 
 Open Scope Z.
 
-Local Ltac solve_montgomery_step_gen_Zlength :=
+Local Ltac solve_small_step_Zlength :=
   intros;
-  rewrite /montgomery_step_gen;
-  rewrite /get_a /get_b /get_c /get_d /get_e /get_f;
+  rewrite /fa /fb /fc /fd /fe /ff;
   repeat match goal with
     | _ => orewrite Sel25519_Zlength
     | _ => orewrite M_Zlength
@@ -264,73 +153,36 @@ Local Ltac solve_montgomery_step_gen_Zlength :=
     | _ => orewrite Zub_Zlength
   end ; reflexivity.
 
-Lemma get_a_montgomery_step_gen_Zlength : forall z a b c d e f x n,
-  Zlength a = 16 -> Zlength b = 16 -> Zlength c = 16 ->
-  Zlength d = 16 -> Zlength x = 16 ->
-  Zlength (get_a (montgomery_step_gen n z a b c d e f x)) = 16.
-Proof. solve_montgomery_step_gen_Zlength. Qed.
-Lemma get_b_montgomery_step_gen_Zlength : forall z a b c d e f x n,
-  Zlength a = 16 -> Zlength b = 16 -> Zlength c = 16 ->
-  Zlength d = 16 -> Zlength x = 16 ->
-  Zlength (get_b (montgomery_step_gen n z a b c d e f x)) = 16.
-Proof. solve_montgomery_step_gen_Zlength. Qed.
-Lemma get_c_montgomery_step_gen_Zlength : forall z a b c d e f x n,
-  Zlength a = 16 -> Zlength b = 16 -> Zlength c = 16 ->
-  Zlength d = 16 -> Zlength x = 16 ->
-  Zlength (get_c (montgomery_step_gen n z a b c d e f x)) = 16.
-Proof. solve_montgomery_step_gen_Zlength. Qed.
-Lemma get_d_montgomery_step_gen_Zlength : forall z a b c d e f x n,
-  Zlength a = 16 -> Zlength b = 16 -> Zlength c = 16 ->
-  Zlength d = 16 -> Zlength x = 16 ->
-  Zlength (get_d (montgomery_step_gen n z a b c d e f x)) = 16.
-Proof. solve_montgomery_step_gen_Zlength. Qed.
-Lemma get_e_montgomery_step_gen_Zlength : forall z a b c d e f x n,
-  Zlength a = 16 -> Zlength b = 16 -> Zlength c = 16 ->
-  Zlength d = 16 -> Zlength x = 16 ->
-  Zlength (get_e (montgomery_step_gen n z a b c d e f x)) = 16.
-Proof. solve_montgomery_step_gen_Zlength. Qed.
-Lemma get_f_montgomery_step_gen_Zlength : forall z a b c d e f x n,
-  Zlength a = 16 -> Zlength b = 16 -> Zlength c = 16 ->
-  Zlength d = 16 -> Zlength x = 16 ->
-  Zlength (get_f (montgomery_step_gen n z a b c d e f x)) = 16.
-Proof. solve_montgomery_step_gen_Zlength. Qed.
-
-Lemma get_a_montgomery_rec_gen_Zlength : forall n z a b c d e f x,
+Lemma fa_Zlength : forall r a b c d e f x,
   Zlength a = 16 -> Zlength b = 16 -> Zlength c = 16 ->
   Zlength d = 16 -> Zlength e = 16 -> Zlength f = 16 -> Zlength x = 16 ->
-  Zlength (get_a (montgomery_rec_gen n z a b c d e f x)) = 16.
-Proof. induction n; intros ; [assumption|] ; simpl.
-apply IHn ; try assumption ; solve_montgomery_step_gen_Zlength. Qed.
-Lemma get_b_montgomery_rec_gen_Zlength : forall n z a b c d e f x,
+  Zlength (fa r a b c d e f x) = 16.
+Proof. solve_small_step_Zlength. Qed.
+Lemma fb_Zlength : forall r a b c d e f x,
   Zlength a = 16 -> Zlength b = 16 -> Zlength c = 16 ->
   Zlength d = 16 -> Zlength e = 16 -> Zlength f = 16 -> Zlength x = 16 ->
-  Zlength (get_b (montgomery_rec_gen n z a b c d e f x)) = 16.
-Proof. induction n; intros ; [assumption|] ; simpl.
-apply IHn ; try assumption ; solve_montgomery_step_gen_Zlength. Qed.
-Lemma get_c_montgomery_rec_gen_Zlength : forall n z a b c d e f x,
+  Zlength (fb r a b c d e f x) = 16.
+Proof. solve_small_step_Zlength. Qed.
+Lemma fc_Zlength : forall r a b c d e f x,
   Zlength a = 16 -> Zlength b = 16 -> Zlength c = 16 ->
   Zlength d = 16 -> Zlength e = 16 -> Zlength f = 16 -> Zlength x = 16 ->
-  Zlength (get_c (montgomery_rec_gen n z a b c d e f x)) = 16.
-Proof. induction n; intros ; [assumption|] ; simpl.
-apply IHn ; try assumption ; solve_montgomery_step_gen_Zlength. Qed.
-Lemma get_d_montgomery_rec_gen_Zlength : forall n z a b c d e f x,
+  Zlength (fc r a b c d e f x) = 16.
+Proof. solve_small_step_Zlength. Qed.
+Lemma fd_Zlength : forall r a b c d e f x,
   Zlength a = 16 -> Zlength b = 16 -> Zlength c = 16 ->
   Zlength d = 16 -> Zlength e = 16 -> Zlength f = 16 -> Zlength x = 16 ->
-  Zlength (get_d (montgomery_rec_gen n z a b c d e f x)) = 16.
-Proof. induction n; intros ; [assumption|] ; simpl.
-apply IHn ; try assumption ; solve_montgomery_step_gen_Zlength. Qed.
-Lemma get_e_montgomery_rec_gen_Zlength : forall n z a b c d e f x,
+  Zlength (fd r a b c d e f x) = 16.
+Proof. solve_small_step_Zlength. Qed.
+Lemma fe_Zlength : forall r a b c d e f x,
   Zlength a = 16 -> Zlength b = 16 -> Zlength c = 16 ->
   Zlength d = 16 -> Zlength e = 16 -> Zlength f = 16 -> Zlength x = 16 ->
-  Zlength (get_e (montgomery_rec_gen n z a b c d e f x)) = 16.
-Proof. induction n; intros ; [assumption|] ; simpl.
-apply IHn ; try assumption ; solve_montgomery_step_gen_Zlength. Qed.
-Lemma get_f_montgomery_rec_gen_Zlength : forall n z a b c d e f x,
+  Zlength (fe r a b c d e f x) = 16.
+Proof. solve_small_step_Zlength. Qed.
+Lemma ff_Zlength : forall r a b c d e f x,
   Zlength a = 16 -> Zlength b = 16 -> Zlength c = 16 ->
   Zlength d = 16 -> Zlength e = 16 -> Zlength f = 16 -> Zlength x = 16 ->
-  Zlength (get_f (montgomery_rec_gen n z a b c d e f x)) = 16.
-Proof. induction n; intros ; [assumption|] ; simpl.
-apply IHn ; try assumption ; solve_montgomery_step_gen_Zlength. Qed.
+  Zlength (ff r a b c d e f x) = 16.
+Proof. solve_small_step_Zlength. Qed.
 
 Variable M_bound_Zlength : forall a b,
   Zlength a = 16 ->
@@ -396,7 +248,7 @@ Local Ltac Simplify_this :=
 change (2^16) with 65536 in *;
 change (2^26) with 67108864 in *.
 
-Lemma get_a_montgomery_step_bound : forall n z a b c d e f x,
+Lemma fa_step_bound : forall r a b c d e f x,
   Zlength a = 16 ->
   Zlength b = 16 ->
   Zlength c = 16 ->
@@ -406,29 +258,29 @@ Lemma get_a_montgomery_step_bound : forall n z a b c d e f x,
     Forall (fun x => -38 <= x < 2^16 + 38) b ->
     Forall (fun x => -38 <= x < 2^16 + 38) c ->
     Forall (fun x => -38 <= x < 2^16 + 38) d ->
-    Forall (fun x => -38 <= x < 2^16 + 38) (get_a (montgomery_step_gen  n z a b c d e f x)).
+    Forall (fun x => -38 <= x < 2^16 + 38) (fa r a b c d e f x).
 Proof.
   intros ; simpl.
   apply Sel25519_bound_lt_le_id.
   apply M_bound_Zlength.
-  solve_montgomery_step_gen_Zlength.
-  solve_montgomery_step_gen_Zlength.
+  solve_small_step_Zlength.
+  solve_small_step_Zlength.
   eapply list.Forall_impl.
   apply Sq_bound_Zlength.
-  solve_montgomery_step_gen_Zlength.
+  solve_small_step_Zlength.
   eapply list.Forall_impl.
   apply A_bound_Zlength_le.
-  solve_montgomery_step_gen_Zlength.
+  solve_small_step_Zlength.
   apply Sel25519_bound_le_lt_trans_le_id ; eauto.
   apply Sel25519_bound_le_lt_trans_le_id ; eauto.
   intros h Hh; simpl in Hh; Simplify_this; omega.
   intros h Hh; simpl in Hh; Simplify_this; omega.
   eapply list.Forall_impl.
   apply Sq_bound_Zlength.
-  solve_montgomery_step_gen_Zlength.
+  solve_small_step_Zlength.
   eapply list.Forall_impl.
   apply Zub_bound_Zlength_lt.
-  solve_montgomery_step_gen_Zlength.
+  solve_small_step_Zlength.
   apply (Sel25519_bound_lt_lt_id (-39) (2 ^ 16 + 38)).
   eapply list.Forall_impl ; eauto ; simpl ; intros ; omega.
   eapply list.Forall_impl ; eauto ; simpl ; intros ; omega.
@@ -438,17 +290,17 @@ Proof.
   intros h Hh; Simplify_this; simpl in Hh; omega.
   intros h Hh; Simplify_this; simpl in Hh; omega.
   apply Sq_bound_Zlength.
-  solve_montgomery_step_gen_Zlength.
+  solve_small_step_Zlength.
   eapply list.Forall_impl.
   apply (A_bound_Zlength_lt (-39) (2^16+ 38) (-39) (2^16+ 38)).
-  solve_montgomery_step_gen_Zlength.
+  solve_small_step_Zlength.
   eapply list.Forall_impl.
   apply M_bound_Zlength.
-  solve_montgomery_step_gen_Zlength.
-  solve_montgomery_step_gen_Zlength.
+  solve_small_step_Zlength.
+  solve_small_step_Zlength.
   eapply list.Forall_impl.
   apply A_bound_Zlength_lt.
-  solve_montgomery_step_gen_Zlength.
+  solve_small_step_Zlength.
   apply (Sel25519_bound_lt_lt_id (-39) (2 ^ 16 + 38)).
   eapply list.Forall_impl ; eauto ; simpl ; intros ; omega.
   eapply list.Forall_impl ; eauto ; simpl ; intros ; omega.
@@ -458,7 +310,7 @@ Proof.
   intros h Hh; Simplify_this; simpl in Hh; omega.
   eapply list.Forall_impl.
   apply Zub_bound_Zlength_lt.
-  solve_montgomery_step_gen_Zlength.
+  solve_small_step_Zlength.
   apply (Sel25519_bound_lt_lt_id (-39) (2 ^ 16 + 38)).
   eapply list.Forall_impl ; eauto ; simpl ; intros ; omega.
   eapply list.Forall_impl ; eauto ; simpl ; intros ; omega.
@@ -469,11 +321,11 @@ Proof.
   intros h Hh; Simplify_this; simpl in Hh; omega.
   eapply list.Forall_impl.
   eapply M_bound_Zlength.
-  solve_montgomery_step_gen_Zlength.
-  solve_montgomery_step_gen_Zlength.
+  solve_small_step_Zlength.
+  solve_small_step_Zlength.
   eapply list.Forall_impl.
   apply Zub_bound_Zlength_lt.
-  solve_montgomery_step_gen_Zlength.
+  solve_small_step_Zlength.
   apply (Sel25519_bound_lt_lt_id (-39) (2 ^ 16 + 38)).
   eapply list.Forall_impl ; eauto ; simpl ; intros ; omega.
   eapply list.Forall_impl ; eauto ; simpl ; intros ; omega.
@@ -483,7 +335,7 @@ Proof.
   intros h Hh; Simplify_this; simpl in Hh; omega.
   eapply list.Forall_impl.
   apply A_bound_Zlength_lt.
-  solve_montgomery_step_gen_Zlength.
+  solve_small_step_Zlength.
   apply (Sel25519_bound_lt_lt_id (-39) (2 ^ 16 + 38)).
   eapply list.Forall_impl ; eauto ; simpl ; intros ; omega.
   eapply list.Forall_impl ; eauto ; simpl ; intros ; omega.
@@ -495,7 +347,7 @@ Proof.
   intros h Hh; Simplify_this; simpl in Hh; omega.
 Qed.
 
-Lemma get_b_montgomery_step_bound : forall n z a b c d e f x,
+Lemma fb_step_bound : forall r a b c d e f x,
   Zlength a = 16 ->
   Zlength b = 16 ->
   Zlength c = 16 ->
@@ -505,23 +357,23 @@ Lemma get_b_montgomery_step_bound : forall n z a b c d e f x,
     Forall (fun x => -38 <= x < 2^16 + 38) b ->
     Forall (fun x => -38 <= x < 2^16 + 38) c ->
     Forall (fun x => -38 <= x < 2^16 + 38) d ->
-    Forall (fun x => -38 <= x < 2^16 + 38) (get_b (montgomery_step_gen  n z a b c d e f x)).
+    Forall (fun x => -38 <= x < 2^16 + 38) (fb r a b c d e f x).
 Proof.
   intros.
   simpl.
   apply Sel25519_bound_lt_le_id.
   apply Sq_bound_Zlength.
-  solve_montgomery_step_gen_Zlength.
+  solve_small_step_Zlength.
   eapply list.Forall_impl.
   apply (A_bound_Zlength_lt (-39) (2^16+ 38) (-39) (2^16+ 38)).
-  solve_montgomery_step_gen_Zlength.
+  solve_small_step_Zlength.
   eapply list.Forall_impl.
   apply M_bound_Zlength.
-  solve_montgomery_step_gen_Zlength.
-  solve_montgomery_step_gen_Zlength.
+  solve_small_step_Zlength.
+  solve_small_step_Zlength.
   eapply list.Forall_impl.
   apply A_bound_Zlength_lt.
-  solve_montgomery_step_gen_Zlength.
+  solve_small_step_Zlength.
   apply (Sel25519_bound_lt_lt_id (-39) (2 ^ 16 + 38)).
   eapply list.Forall_impl ; eauto ; simpl ; intros ; omega.
   eapply list.Forall_impl ; eauto ; simpl ; intros ; omega.
@@ -531,7 +383,7 @@ Proof.
   intros h Hh; Simplify_this; simpl in Hh; omega.
   eapply list.Forall_impl.
   apply Zub_bound_Zlength_lt.
-  solve_montgomery_step_gen_Zlength.
+  solve_small_step_Zlength.
   apply (Sel25519_bound_lt_lt_id (-39) (2 ^ 16 + 38)).
   eapply list.Forall_impl ; eauto ; simpl ; intros ; omega.
   eapply list.Forall_impl ; eauto ; simpl ; intros ; omega.
@@ -542,11 +394,11 @@ Proof.
   intros h Hh; Simplify_this; simpl in Hh; omega.
   eapply list.Forall_impl.
   apply M_bound_Zlength.
-  solve_montgomery_step_gen_Zlength.
-  solve_montgomery_step_gen_Zlength.
+  solve_small_step_Zlength.
+  solve_small_step_Zlength.
   eapply list.Forall_impl.
   apply Zub_bound_Zlength_lt.
-  solve_montgomery_step_gen_Zlength.
+  solve_small_step_Zlength.
   apply (Sel25519_bound_lt_lt_id (-39) (2 ^ 16 + 38)).
   eapply list.Forall_impl ; eauto ; simpl ; intros ; omega.
   eapply list.Forall_impl ; eauto ; simpl ; intros ; omega.
@@ -556,7 +408,7 @@ Proof.
   intros h Hh; Simplify_this; simpl in Hh; omega.
   eapply list.Forall_impl.
   apply A_bound_Zlength_lt.
-  solve_montgomery_step_gen_Zlength.
+  solve_small_step_Zlength.
   apply (Sel25519_bound_lt_lt_id (-39) (2 ^ 16 + 38)).
   eapply list.Forall_impl ; eauto ; simpl ; intros ; omega.
   eapply list.Forall_impl ; eauto ; simpl ; intros ; omega.
@@ -567,14 +419,14 @@ Proof.
   intros h Hh; Simplify_this; simpl in Hh; omega.
   intros h Hh; Simplify_this; simpl in Hh; omega.
   apply M_bound_Zlength.
-  solve_montgomery_step_gen_Zlength.
-  solve_montgomery_step_gen_Zlength.
+  solve_small_step_Zlength.
+  solve_small_step_Zlength.
   eapply list.Forall_impl.
   apply Sq_bound_Zlength.
-  solve_montgomery_step_gen_Zlength.
+  solve_small_step_Zlength.
   eapply list.Forall_impl.
   apply (A_bound_Zlength_lt (-39) (2^16+ 38) (-39) (2^16+ 38)).
-  solve_montgomery_step_gen_Zlength.
+  solve_small_step_Zlength.
   apply (Sel25519_bound_lt_lt_id (-39) (2 ^ 16 + 38)).
   eapply list.Forall_impl ; eauto ; simpl ; intros ; omega.
   eapply list.Forall_impl ; eauto ; simpl ; intros ; omega.
@@ -585,10 +437,10 @@ Proof.
   intros h Hh; Simplify_this; simpl in Hh; omega.
   eapply list.Forall_impl.
   apply Sq_bound_Zlength.
-  solve_montgomery_step_gen_Zlength.
+  solve_small_step_Zlength.
   eapply list.Forall_impl.
   apply (Zub_bound_Zlength_lt (-39) (2^16+ 38) (-39) (2^16+ 38)).
-  solve_montgomery_step_gen_Zlength.
+  solve_small_step_Zlength.
   apply (Sel25519_bound_lt_lt_id (-39) (2 ^ 16 + 38)).
   eapply list.Forall_impl ; eauto ; simpl ; intros ; omega.
   eapply list.Forall_impl ; eauto ; simpl ; intros ; omega.
@@ -600,7 +452,7 @@ Proof.
 Qed.
 
 
-Lemma get_c_montgomery_step_bound : forall n z a b c d e f x,
+Lemma fc_step_bound : forall r a b c d e f x,
   Zlength a = 16 ->
   Zlength b = 16 ->
   Zlength c = 16 ->
@@ -611,33 +463,33 @@ Lemma get_c_montgomery_step_bound : forall n z a b c d e f x,
     Forall (fun x => -38 <= x < 2^16 + 38) c ->
     Forall (fun x => -38 <= x < 2^16 + 38) d ->
     Forall (fun x => -38 <= x < 2^16 + 38) x ->
-    Forall (fun x => -38 <= x < 2^16 + 38) (get_c (montgomery_step_gen  n z a b c d e f x)).
+    Forall (fun x => -38 <= x < 2^16 + 38) (fc r a b c d e f x).
 Proof.
   intros.
   simpl.
   apply Sel25519_bound_lt_le_id.
   apply M_bound_Zlength.
-  solve_montgomery_step_gen_Zlength.
-  solve_montgomery_step_gen_Zlength.
+  solve_small_step_Zlength.
+  solve_small_step_Zlength.
   eapply list.Forall_impl.
   apply (Zub_bound_Zlength_lt (-39) (2^16+ 38) (-39) (2^16+ 38)).
-  solve_montgomery_step_gen_Zlength.
+  solve_small_step_Zlength.
   eapply list.Forall_impl.
   apply Sq_bound_Zlength.
-  solve_montgomery_step_gen_Zlength.
+  solve_small_step_Zlength.
   eapply list.Forall_impl.
   apply A_bound_Zlength_le.
-  solve_montgomery_step_gen_Zlength.
+  solve_small_step_Zlength.
   apply Sel25519_bound_le_lt_trans_le_id ; eauto.
   apply Sel25519_bound_le_lt_trans_le_id ; eauto.
   intros h Hh; simpl in Hh; Simplify_this; omega.
   intros h Hh; simpl in Hh; Simplify_this; omega.
   eapply list.Forall_impl.
   apply Sq_bound_Zlength.
-  solve_montgomery_step_gen_Zlength.
+  solve_small_step_Zlength.
   eapply list.Forall_impl.
   apply Zub_bound_Zlength_lt.
-  solve_montgomery_step_gen_Zlength.
+  solve_small_step_Zlength.
   apply (Sel25519_bound_lt_lt_id (-39) (2 ^ 16 + 38)).
   eapply list.Forall_impl ; eauto ; simpl ; intros ; omega.
   eapply list.Forall_impl ; eauto ; simpl ; intros ; omega.
@@ -649,20 +501,20 @@ Proof.
   intros h Hh; Simplify_this; simpl in Hh; omega.
   eapply list.Forall_impl.
   apply (A_bound_Zlength_lt (-39) (2^16+ 38) (-39) (2^16+ 38)).
-  solve_montgomery_step_gen_Zlength.
+  solve_small_step_Zlength.
   eapply list.Forall_impl.
   apply M_bound_Zlength.
-  solve_montgomery_step_gen_Zlength.
+  solve_small_step_Zlength.
   assumption.
   eapply list.Forall_impl.
   apply (Zub_bound_Zlength_lt (-39) (2^16+ 38) (-39) (2^16+ 38)).
-  solve_montgomery_step_gen_Zlength.
+  solve_small_step_Zlength.
   eapply list.Forall_impl.
   apply Sq_bound_Zlength.
-  solve_montgomery_step_gen_Zlength.
+  solve_small_step_Zlength.
   eapply list.Forall_impl.
   apply (A_bound_Zlength_lt (-39) (2^16+ 38) (-39) (2^16+ 38)).
-  solve_montgomery_step_gen_Zlength.
+  solve_small_step_Zlength.
   apply (Sel25519_bound_lt_lt_id (-39) (2 ^ 16 + 38)).
   eapply list.Forall_impl ; eauto ; simpl ; intros ; omega.
   eapply list.Forall_impl ; eauto ; simpl ; intros ; omega.
@@ -673,10 +525,10 @@ Proof.
   intros h Hh; Simplify_this; simpl in Hh; omega.
   eapply list.Forall_impl.
   eapply Sq_bound_Zlength.
-  solve_montgomery_step_gen_Zlength.
+  solve_small_step_Zlength.
   eapply list.Forall_impl.
   apply (Zub_bound_Zlength_lt (-39) (2^16+ 38) (-39) (2^16+ 38)).
-  solve_montgomery_step_gen_Zlength.
+  solve_small_step_Zlength.
   apply (Sel25519_bound_lt_lt_id (-39) (2 ^ 16 + 38)).
   eapply list.Forall_impl ; eauto ; simpl ; intros ; omega.
   eapply list.Forall_impl ; eauto ; simpl ; intros ; omega.
@@ -692,10 +544,10 @@ Proof.
   intros h Hh; Simplify_this; simpl in Hh; omega.
   eapply list.Forall_impl.
   apply Sq_bound_Zlength.
-  solve_montgomery_step_gen_Zlength.
+  solve_small_step_Zlength.
   eapply list.Forall_impl.
   apply (A_bound_Zlength_lt (-39) (2^16+ 38) (-39) (2^16+ 38)).
-  solve_montgomery_step_gen_Zlength.
+  solve_small_step_Zlength.
   apply (Sel25519_bound_lt_lt_id (-39) (2 ^ 16 + 38)).
   eapply list.Forall_impl ; eauto ; simpl ; intros ; omega.
   eapply list.Forall_impl ; eauto ; simpl ; intros ; omega.
@@ -706,21 +558,21 @@ Proof.
   intros h Hh; Simplify_this; simpl in Hh; omega.
   intros h Hh; Simplify_this; simpl in Hh; omega.
   apply M_bound_Zlength.
-  solve_montgomery_step_gen_Zlength.
+  solve_small_step_Zlength.
   assumption.
   eapply list.Forall_impl.
   apply Sq_bound_Zlength.
-  solve_montgomery_step_gen_Zlength.
+  solve_small_step_Zlength.
   eapply list.Forall_impl.
   apply (Zub_bound_Zlength_lt (-39) (2^16+ 38) (-39) (2^16+ 38)).
-  solve_montgomery_step_gen_Zlength.
+  solve_small_step_Zlength.
   eapply list.Forall_impl.
   apply M_bound_Zlength.
-  solve_montgomery_step_gen_Zlength.
-  solve_montgomery_step_gen_Zlength.
+  solve_small_step_Zlength.
+  solve_small_step_Zlength.
   eapply list.Forall_impl.
   apply (A_bound_Zlength_lt (-39) (2^16+ 38) (-39) (2^16+ 38)).
-  solve_montgomery_step_gen_Zlength.
+  solve_small_step_Zlength.
   apply (Sel25519_bound_lt_lt_id (-39) (2 ^ 16 + 38)).
   eapply list.Forall_impl ; eauto ; simpl ; intros ; omega.
   eapply list.Forall_impl ; eauto ; simpl ; intros ; omega.
@@ -730,7 +582,7 @@ Proof.
   intros h Hh; Simplify_this; simpl in Hh; omega.
   eapply list.Forall_impl.
   apply (Zub_bound_Zlength_lt (-39) (2^16+ 38) (-39) (2^16+ 38)).
-  solve_montgomery_step_gen_Zlength.
+  solve_small_step_Zlength.
   apply (Sel25519_bound_lt_lt_id (-39) (2 ^ 16 + 38)).
   eapply list.Forall_impl ; eauto ; simpl ; intros ; omega.
   eapply list.Forall_impl ; eauto ; simpl ; intros ; omega.
@@ -741,11 +593,11 @@ Proof.
   intros h Hh; Simplify_this; simpl in Hh; omega.
   eapply list.Forall_impl.
   apply M_bound_Zlength.
-  solve_montgomery_step_gen_Zlength.
-  solve_montgomery_step_gen_Zlength.
+  solve_small_step_Zlength.
+  solve_small_step_Zlength.
   eapply list.Forall_impl.
   apply (Zub_bound_Zlength_lt (-39) (2^16+ 38) (-39) (2^16+ 38)).
-  solve_montgomery_step_gen_Zlength.
+  solve_small_step_Zlength.
   apply (Sel25519_bound_lt_lt_id (-39) (2 ^ 16 + 38)).
   eapply list.Forall_impl ; eauto ; simpl ; intros ; omega.
   eapply list.Forall_impl ; eauto ; simpl ; intros ; omega.
@@ -755,7 +607,7 @@ Proof.
   intros h Hh; Simplify_this; simpl in Hh; omega.
   eapply list.Forall_impl.
   apply (A_bound_Zlength_lt (-39) (2^16+ 38) (-39) (2^16+ 38)).
-  solve_montgomery_step_gen_Zlength.
+  solve_small_step_Zlength.
   apply (Sel25519_bound_lt_lt_id (-39) (2 ^ 16 + 38)).
   eapply list.Forall_impl ; eauto ; simpl ; intros ; omega.
   eapply list.Forall_impl ; eauto ; simpl ; intros ; omega.
@@ -770,7 +622,7 @@ Proof.
   intros h Hh; Simplify_this; simpl in Hh; omega.
 Qed.
 
-Lemma get_d_montgomery_step_bound : forall n z a b c d e f x,
+Lemma fd_step_bound : forall r a b c d e f x,
   Zlength a = 16 ->
   Zlength b = 16 ->
   Zlength c = 16 ->
@@ -781,27 +633,27 @@ Lemma get_d_montgomery_step_bound : forall n z a b c d e f x,
     Forall (fun x => -38 <= x < 2^16 + 38) c ->
     Forall (fun x => -38 <= x < 2^16 + 38) d ->
     Forall (fun x => -38 <= x < 2^16 + 38) x ->
-    Forall (fun x => -38 <= x < 2^16 + 38) (get_d (montgomery_step_gen  n z a b c d e f x)).
+    Forall (fun x => -38 <= x < 2^16 + 38) (fd r a b c d e f x).
 Proof.
   intros.
   simpl.
   apply Sel25519_bound_lt_le_id.
   apply M_bound_Zlength.
-  solve_montgomery_step_gen_Zlength.
+  solve_small_step_Zlength.
   assumption.
   eapply list.Forall_impl.
   apply Sq_bound_Zlength.
-  solve_montgomery_step_gen_Zlength.
+  solve_small_step_Zlength.
   eapply list.Forall_impl.
   apply (Zub_bound_Zlength_lt (-39) (2^16+ 38) (-39) (2^16+ 38)).
-  solve_montgomery_step_gen_Zlength.
+  solve_small_step_Zlength.
   eapply list.Forall_impl.
   apply M_bound_Zlength.
-  solve_montgomery_step_gen_Zlength.
-  solve_montgomery_step_gen_Zlength.
+  solve_small_step_Zlength.
+  solve_small_step_Zlength.
   eapply list.Forall_impl.
   apply (A_bound_Zlength_lt (-39) (2^16+ 38) (-39) (2^16+ 38)).
-  solve_montgomery_step_gen_Zlength.
+  solve_small_step_Zlength.
   apply (Sel25519_bound_lt_lt_id (-39) (2 ^ 16 + 38)).
   eapply list.Forall_impl ; eauto ; simpl ; intros ; omega.
   eapply list.Forall_impl ; eauto ; simpl ; intros ; omega.
@@ -811,7 +663,7 @@ Proof.
   intros h Hh; simpl in Hh; Simplify_this; omega.
   eapply list.Forall_impl.
   apply (Zub_bound_Zlength_lt (-39) (2^16+ 38) (-39) (2^16+ 38)).
-  solve_montgomery_step_gen_Zlength.
+  solve_small_step_Zlength.
   apply (Sel25519_bound_lt_lt_id (-39) (2 ^ 16 + 38)).
   eapply list.Forall_impl ; eauto ; simpl ; intros ; omega.
   eapply list.Forall_impl ; eauto ; simpl ; intros ; omega.
@@ -822,11 +674,11 @@ Proof.
   intros h Hh; Simplify_this; simpl in Hh; omega.
   eapply list.Forall_impl.
   apply M_bound_Zlength.
-  solve_montgomery_step_gen_Zlength.
-  solve_montgomery_step_gen_Zlength.
+  solve_small_step_Zlength.
+  solve_small_step_Zlength.
   eapply list.Forall_impl.
   apply (Zub_bound_Zlength_lt (-39) (2^16+ 38) (-39) (2^16+ 38)).
-  solve_montgomery_step_gen_Zlength.
+  solve_small_step_Zlength.
   apply (Sel25519_bound_lt_lt_id (-39) (2 ^ 16 + 38)).
   eapply list.Forall_impl ; eauto ; simpl ; intros ; omega.
   eapply list.Forall_impl ; eauto ; simpl ; intros ; omega.
@@ -836,7 +688,7 @@ Proof.
   intros h Hh; Simplify_this; simpl in Hh; omega.
   eapply list.Forall_impl.
   apply (A_bound_Zlength_lt (-39) (2^16+ 38) (-39) (2^16+ 38)).
-  solve_montgomery_step_gen_Zlength.
+  solve_small_step_Zlength.
   apply (Sel25519_bound_lt_lt_id (-39) (2 ^ 16 + 38)).
   eapply list.Forall_impl ; eauto ; simpl ; intros ; omega.
   eapply list.Forall_impl ; eauto ; simpl ; intros ; omega.
@@ -850,17 +702,17 @@ Proof.
   eapply list.Forall_impl ; eauto.
   intros h Hh; Simplify_this; simpl in Hh; omega.
   apply M_bound_Zlength.
-  solve_montgomery_step_gen_Zlength.
-  solve_montgomery_step_gen_Zlength.
+  solve_small_step_Zlength.
+  solve_small_step_Zlength.
   eapply list.Forall_impl.
   apply (Zub_bound_Zlength_lt (-39) (2^16+ 38) (-39) (2^16+ 38)).
-  solve_montgomery_step_gen_Zlength.
+  solve_small_step_Zlength.
   eapply list.Forall_impl.
   apply Sq_bound_Zlength.
-  solve_montgomery_step_gen_Zlength.
+  solve_small_step_Zlength.
   eapply list.Forall_impl.
   apply (A_bound_Zlength_lt (-39) (2^16+ 38) (-39) (2^16+ 38)).
-  solve_montgomery_step_gen_Zlength.
+  solve_small_step_Zlength.
   apply (Sel25519_bound_lt_lt_id (-39) (2 ^ 16 + 38)).
   eapply list.Forall_impl ; eauto ; simpl ; intros ; omega.
   eapply list.Forall_impl ; eauto ; simpl ; intros ; omega.
@@ -871,10 +723,10 @@ Proof.
   intros h Hh; Simplify_this; simpl in Hh; omega.
   eapply list.Forall_impl.
   apply Sq_bound_Zlength.
-  solve_montgomery_step_gen_Zlength.
+  solve_small_step_Zlength.
   eapply list.Forall_impl.
   apply (Zub_bound_Zlength_lt (-39) (2^16+ 38) (-39) (2^16+ 38)).
-  solve_montgomery_step_gen_Zlength.
+  solve_small_step_Zlength.
   apply (Sel25519_bound_lt_lt_id (-39) (2 ^ 16 + 38)).
   eapply list.Forall_impl ; eauto ; simpl ; intros ; omega.
   eapply list.Forall_impl ; eauto ; simpl ; intros ; omega.
@@ -886,20 +738,20 @@ Proof.
   intros h Hh; Simplify_this; simpl in Hh; omega.
   eapply list.Forall_impl.
   apply (A_bound_Zlength_lt (-39) (2^16+ 38) (-39) (2^16+ 38)).
-  solve_montgomery_step_gen_Zlength.
+  solve_small_step_Zlength.
   eapply list.Forall_impl.
   apply M_bound_Zlength.
-  solve_montgomery_step_gen_Zlength.
+  solve_small_step_Zlength.
   apply _121665_Zlength.
   eapply list.Forall_impl.
   apply (Zub_bound_Zlength_lt (-39) (2^16+ 38) (-39) (2^16+ 38)).
-  solve_montgomery_step_gen_Zlength.
+  solve_small_step_Zlength.
   eapply list.Forall_impl.
   apply Sq_bound_Zlength.
-  solve_montgomery_step_gen_Zlength.
+  solve_small_step_Zlength.
   eapply list.Forall_impl.
   apply (A_bound_Zlength_lt (-39) (2^16+ 38) (-39) (2^16+ 38)).
-  solve_montgomery_step_gen_Zlength.
+  solve_small_step_Zlength.
   apply (Sel25519_bound_lt_lt_id (-39) (2 ^ 16 + 38)).
   eapply list.Forall_impl ; eauto ; simpl ; intros ; omega.
   eapply list.Forall_impl ; eauto ; simpl ; intros ; omega.
@@ -910,10 +762,10 @@ Proof.
   intros h Hh; Simplify_this; simpl in Hh; omega.
   eapply list.Forall_impl.
   apply Sq_bound_Zlength.
-  solve_montgomery_step_gen_Zlength.
+  solve_small_step_Zlength.
   eapply list.Forall_impl.
   apply (Zub_bound_Zlength_lt (-39) (2^16+ 38) (-39) (2^16+ 38)).
-  solve_montgomery_step_gen_Zlength.
+  solve_small_step_Zlength.
   apply (Sel25519_bound_lt_lt_id (-39) (2 ^ 16 + 38)).
   eapply list.Forall_impl ; eauto ; simpl ; intros ; omega.
   eapply list.Forall_impl ; eauto ; simpl ; intros ; omega.
@@ -929,10 +781,10 @@ Proof.
   intros h Hh; Simplify_this; simpl in Hh; omega.
   eapply list.Forall_impl.
   apply Sq_bound_Zlength.
-  solve_montgomery_step_gen_Zlength.
+  solve_small_step_Zlength.
   eapply list.Forall_impl.
   apply (A_bound_Zlength_lt (-39) (2^16+ 38) (-39) (2^16+ 38)).
-  solve_montgomery_step_gen_Zlength.
+  solve_small_step_Zlength.
   apply (Sel25519_bound_lt_lt_id (-39) (2 ^ 16 + 38)).
   eapply list.Forall_impl ; eauto ; simpl ; intros ; omega.
   eapply list.Forall_impl ; eauto ; simpl ; intros ; omega.
@@ -944,169 +796,6 @@ Proof.
   intros h Hh; Simplify_this; simpl in Hh; omega.
 Qed.
 
-Lemma get_e_montgomery_step_bound : forall n z a b c d e f x,
-  Zlength a = 16 ->
-  Zlength b = 16 ->
-  Zlength c = 16 ->
-  Zlength d = 16 ->
-  Zlength x = 16 ->
-    Forall (fun x => -38 <= x < 2^16 + 38) a ->
-    Forall (fun x => -38 <= x < 2^16 + 38) b ->
-    Forall (fun x => -38 <= x < 2^16 + 38) c ->
-    Forall (fun x => -38 <= x < 2^16 + 38) d ->
-    Forall (fun x => -38 <= x < 2^16 + 38) x ->
-    Forall (fun x => -76 <= x < 2^17 + 76) (get_e (montgomery_step_gen  n z a b c d e f x)).
-Proof.
-  intros.
-  simpl.
-  
-
-Admitted.
-
-Lemma get_f_montgomery_step_bound : forall n z a b c d e f x,
-  Zlength a = 16 ->
-  Zlength b = 16 ->
-  Zlength c = 16 ->
-  Zlength d = 16 ->
-  Zlength x = 16 ->
-    Forall (fun x => -38 <= x < 2^16 + 38) a ->
-    Forall (fun x => -38 <= x < 2^16 + 38) b ->
-    Forall (fun x => -38 <= x < 2^16 + 38) c ->
-    Forall (fun x => -38 <= x < 2^16 + 38) d ->
-    Forall (fun x => -38 <= x < 2^16 + 38) x ->
-    Forall (fun x => -76 <= x < 2^17 + 76) (get_f (montgomery_step_gen  n z a b c d e f x)).
-Proof.
-  intros.
-  simpl.
-
-
-Admitted.
-
-
-Lemma get_a_montgomery_rec_gen_bound : forall n z a b c d e f x,
-  Zlength a = 16 ->
-  Zlength b = 16 ->
-  Zlength c = 16 ->
-  Zlength d = 16 ->
-  Zlength x = 16 ->
-    Forall (fun x => -38 <= x < 2^16 + 38) a ->
-    Forall (fun x => -38 <= x < 2^16 + 38) b ->
-    Forall (fun x => -38 <= x < 2^16 + 38) c ->
-    Forall (fun x => -38 <= x < 2^16 + 38) d ->
-    Forall (fun x => 0 <= x < 2^16) x ->
-    Forall (fun x => -38 <= x < 2^16 + 38) (get_a (montgomery_rec_gen  n z a b c d e f x)).
-Proof.
-induction n ; intros.
-simpl ; auto.
-rewrite opt_montgomery_rec_step_gen.
-apply IHn ; try assumption.
-apply get_a_montgomery_step_gen_Zlength ; auto.
-apply get_b_montgomery_step_gen_Zlength ; auto.
-apply get_c_montgomery_step_gen_Zlength ; auto.
-apply get_d_montgomery_step_gen_Zlength ; auto.
-apply get_a_montgomery_step_bound ; auto.
-apply get_b_montgomery_step_bound ; auto.
-apply get_c_montgomery_step_bound ; auto.
-eapply list.Forall_impl ; eauto.
-intros h Hh; Simplify_this; simpl in Hh; omega.
-apply get_d_montgomery_step_bound ; auto.
-eapply list.Forall_impl ; eauto.
-intros h Hh; Simplify_this; simpl in Hh; omega.
-Qed.
-
-Lemma get_b_montgomery_rec_gen_bound : forall n z a b c d e f x,
-  Zlength a = 16 ->
-  Zlength b = 16 ->
-  Zlength c = 16 ->
-  Zlength d = 16 ->
-  Zlength x = 16 ->
-    Forall (fun x => -38 <= x < 2^16 + 38) a ->
-    Forall (fun x => -38 <= x < 2^16 + 38) b ->
-    Forall (fun x => -38 <= x < 2^16 + 38) c ->
-    Forall (fun x => -38 <= x < 2^16 + 38) d ->
-    Forall (fun x => 0 <= x < 2^16) x ->
-    Forall (fun x => -38 <= x < 2^16 + 38) (get_b (montgomery_rec_gen  n z a b c d e f x)).
-Proof.
-induction n ; intros.
-simpl ; auto.
-rewrite opt_montgomery_rec_step_gen.
-apply IHn ; try assumption.
-apply get_a_montgomery_step_gen_Zlength ; auto.
-apply get_b_montgomery_step_gen_Zlength ; auto.
-apply get_c_montgomery_step_gen_Zlength ; auto.
-apply get_d_montgomery_step_gen_Zlength ; auto.
-apply get_a_montgomery_step_bound ; auto.
-apply get_b_montgomery_step_bound ; auto.
-apply get_c_montgomery_step_bound ; auto.
-eapply list.Forall_impl ; eauto.
-intros h Hh; Simplify_this; simpl in Hh; omega.
-apply get_d_montgomery_step_bound ; auto.
-eapply list.Forall_impl ; eauto.
-intros h Hh; Simplify_this; simpl in Hh; omega.
-Qed.
-
-Lemma get_c_montgomery_rec_gen_bound : forall n z a b c d e f x,
-  Zlength a = 16 ->
-  Zlength b = 16 ->
-  Zlength c = 16 ->
-  Zlength d = 16 ->
-  Zlength x = 16 ->
-    Forall (fun x => -38 <= x < 2^16 + 38) a ->
-    Forall (fun x => -38 <= x < 2^16 + 38) b ->
-    Forall (fun x => -38 <= x < 2^16 + 38) c ->
-    Forall (fun x => -38 <= x < 2^16 + 38) d ->
-    Forall (fun x => 0 <= x < 2^16) x ->
-    Forall (fun x => -38 <= x < 2^16 + 38) (get_c (montgomery_rec_gen  n z a b c d e f x)).
-Proof.
-induction n ; intros.
-simpl ; auto.
-rewrite opt_montgomery_rec_step_gen.
-apply IHn ; try assumption.
-apply get_a_montgomery_step_gen_Zlength ; auto.
-apply get_b_montgomery_step_gen_Zlength ; auto.
-apply get_c_montgomery_step_gen_Zlength ; auto.
-apply get_d_montgomery_step_gen_Zlength ; auto.
-apply get_a_montgomery_step_bound ; auto.
-apply get_b_montgomery_step_bound ; auto.
-apply get_c_montgomery_step_bound ; auto.
-eapply list.Forall_impl ; eauto.
-intros h Hh; Simplify_this; simpl in Hh; omega.
-apply get_d_montgomery_step_bound ; auto.
-eapply list.Forall_impl ; eauto.
-intros h Hh; Simplify_this; simpl in Hh; omega.
-Qed.
-Lemma get_d_montgomery_rec_gen_bound : forall n z a b c d e f x,
-  Zlength a = 16 ->
-  Zlength b = 16 ->
-  Zlength c = 16 ->
-  Zlength d = 16 ->
-  Zlength x = 16 ->
-    Forall (fun x => -38 <= x < 2^16 + 38) a ->
-    Forall (fun x => -38 <= x < 2^16 + 38) b ->
-    Forall (fun x => -38 <= x < 2^16 + 38) c ->
-    Forall (fun x => -38 <= x < 2^16 + 38) d ->
-    Forall (fun x => 0 <= x < 2^16) x ->
-    Forall (fun x => -38 <= x < 2^16 + 38) (get_d (montgomery_rec_gen  n z a b c d e f x)).
-Proof.
-induction n ; intros.
-simpl ; auto.
-rewrite opt_montgomery_rec_step_gen.
-apply IHn ; try assumption.
-apply get_a_montgomery_step_gen_Zlength ; auto.
-apply get_b_montgomery_step_gen_Zlength ; auto.
-apply get_c_montgomery_step_gen_Zlength ; auto.
-apply get_d_montgomery_step_gen_Zlength ; auto.
-apply get_a_montgomery_step_bound ; auto.
-apply get_b_montgomery_step_bound ; auto.
-apply get_c_montgomery_step_bound ; auto.
-eapply list.Forall_impl ; eauto.
-intros h Hh; Simplify_this; simpl in Hh; omega.
-apply get_d_montgomery_step_bound ; auto.
-eapply list.Forall_impl ; eauto.
-intros h Hh; Simplify_this; simpl in Hh; omega.
-Qed.
-
-Close Scope Z.
 End ScalarRec.
 
-
+Close Scope Z.
