Low/Get_abcdef.v
@@ -1,0 +1,38 @@
+Require Import Tweetnacl.Libs.Export.
+
+Definition get_a (t:(list Z * list Z * list Z * list Z * list Z * list Z)) : list Z := match t with
+  (a,b,c,d,e,f) => a
+end.
+Definition get_b (t:(list Z * list Z * list Z * list Z * list Z * list Z)) : list Z := match t with
+  (a,b,c,d,e,f) => b
+end.
+Definition get_c (t:(list Z * list Z * list Z * list Z * list Z * list Z)) : list Z := match t with
+  (a,b,c,d,e,f) => c
+end.
+Definition get_d (t:(list Z * list Z * list Z * list Z * list Z * list Z)) : list Z := match t with
+  (a,b,c,d,e,f) => d
+end.
+Definition get_e (t:(list Z * list Z * list Z * list Z * list Z * list Z)) : list Z := match t with
+  (a,b,c,d,e,f) => e
+end.
+Definition get_f (t:(list Z * list Z * list Z * list Z * list Z * list Z)) : list Z := match t with
+  (a,b,c,d,e,f) => f
+end.
+
+Lemma get_a_length : forall a b c d e f, length (get_a (a,b,c,d,e,f)) = length a. Proof. go. Qed.
+Lemma get_b_length : forall a b c d e f, length (get_b (a,b,c,d,e,f)) = length b. Proof. go. Qed.
+Lemma get_c_length : forall a b c d e f, length (get_c (a,b,c,d,e,f)) = length c. Proof. go. Qed.
+Lemma get_d_length : forall a b c d e f, length (get_d (a,b,c,d,e,f)) = length d. Proof. go. Qed.
+Lemma get_e_length : forall a b c d e f, length (get_e (a,b,c,d,e,f)) = length e. Proof. go. Qed.
+Lemma get_f_length : forall a b c d e f, length (get_f (a,b,c,d,e,f)) = length f. Proof. go. Qed.
+
+Open Scope Z.
+
+Lemma get_a_Zlength : forall a b c d e f, Zlength (get_a (a,b,c,d,e,f)) = Zlength a. Proof. go. Qed.
+Lemma get_b_Zlength : forall a b c d e f, Zlength (get_b (a,b,c,d,e,f)) = Zlength b. Proof. go. Qed.
+Lemma get_c_Zlength : forall a b c d e f, Zlength (get_c (a,b,c,d,e,f)) = Zlength c. Proof. go. Qed.
+Lemma get_d_Zlength : forall a b c d e f, Zlength (get_d (a,b,c,d,e,f)) = Zlength d. Proof. go. Qed.
+Lemma get_e_Zlength : forall a b c d e f, Zlength (get_e (a,b,c,d,e,f)) = Zlength e. Proof. go. Qed.
+Lemma get_f_Zlength : forall a b c d e f, Zlength (get_f (a,b,c,d,e,f)) = Zlength f. Proof. go. Qed.
+
+Close Scope Z.
