Low/ScalarMult_rev_gen.v
@@ -1,0 +1,455 @@
+Require Import Tweetnacl.Libs.Export.
+Require Import Tweetnacl.Low.ScalarMult_gen_small.
+Require Import Tweetnacl.Low.Get_abcdef.
+
+Section ScalarRec.
+
+Variable A : list Z -> list Z -> list Z.
+Variable M : list Z -> list Z -> list Z.
+Variable Zub : list Z -> list Z -> list Z.
+Variable Sq : list Z -> list Z.
+Variable _121665: list Z.
+Variable Sel25519 : Z -> list Z -> list Z -> list Z.
+Variable getbit : Z -> list Z -> Z.
+
+Definition fa := fa A M Zub Sq Sel25519.
+Definition fb := fb A M Zub Sq Sel25519.
+Definition fc := fc A M Zub Sq _121665 Sel25519.
+Definition fd := fd A M Zub Sq _121665 Sel25519.
+Definition fe := fe A M Zub Sel25519.
+Definition ff := ff Zub Sq Sel25519.
+
+Definition step_abstract n z (a b c d e f x:list Z) := let r := getbit (Z.of_nat n) z in
+  (fa r a b c d e f x,
+  fb r a b c d e f x,
+  fc r a b c d e f x,
+  fd r a b c d e f x,
+  fe r a b c d e f x,
+  ff r a b c d e f x).
+
+Fixpoint abstract_rec_rev m p (z a b c d e f x : list Z) : (list Z * list Z * list Z * list Z * list Z * list Z)
+  :=
+  match m with
+  | 0%nat => (a,b,c,d,e,f)
+  | S n => 
+      match (abstract_rec_rev n p z a b c d e f x) with
+        | (a,b,c,d,e,f) =>
+        let r := getbit (Z.of_nat (p - n)) z in
+        (fa r a b c d e f x,
+        fb r a b c d e f x,
+        fc r a b c d e f x,
+        fd r a b c d e f x,
+        fe r a b c d e f x,
+        ff r a b c d e f x)
+      end
+  end.
+
+Lemma abstract_step_rev_a : forall n p (z a b c d e f x : list Z),
+  fa (getbit (Z.of_nat (p - n)) z)
+   (get_a (abstract_rec_rev n p z a b c d e f x))
+   (get_b (abstract_rec_rev n p z a b c d e f x))
+   (get_c (abstract_rec_rev n p z a b c d e f x))
+   (get_d (abstract_rec_rev n p z a b c d e f x))
+   (get_e (abstract_rec_rev n p z a b c d e f x))
+   (get_f (abstract_rec_rev n p z a b c d e f x))
+   x
+  =
+  get_a (abstract_rec_rev (S n) p z a b c d e f x).
+Proof.
+intros; simpl; remember (abstract_rec_rev n p z a b c d e f x) as k.
+destruct k as (((((a0,b0),c0),d0),e0),f0); reflexivity.
+Qed.
+
+Lemma abstract_step_rev_b : forall n p (z a b c d e f x : list Z),
+  fb (getbit (Z.of_nat (p - n)) z)
+   (get_a (abstract_rec_rev n p z a b c d e f x))
+   (get_b (abstract_rec_rev n p z a b c d e f x))
+   (get_c (abstract_rec_rev n p z a b c d e f x))
+   (get_d (abstract_rec_rev n p z a b c d e f x))
+   (get_e (abstract_rec_rev n p z a b c d e f x))
+   (get_f (abstract_rec_rev n p z a b c d e f x))
+   x
+  =
+  get_b (abstract_rec_rev (S n) p z a b c d e f x).
+Proof.
+intros; simpl; remember (abstract_rec_rev n p z a b c d e f x) as k.
+destruct k as (((((a0,b0),c0),d0),e0),f0); reflexivity.
+Qed.
+
+Lemma abstract_step_rev_c : forall n p (z a b c d e f x : list Z),
+  fc (getbit (Z.of_nat (p - n)) z)
+   (get_a (abstract_rec_rev n p z a b c d e f x))
+   (get_b (abstract_rec_rev n p z a b c d e f x))
+   (get_c (abstract_rec_rev n p z a b c d e f x))
+   (get_d (abstract_rec_rev n p z a b c d e f x))
+   (get_e (abstract_rec_rev n p z a b c d e f x))
+   (get_f (abstract_rec_rev n p z a b c d e f x))
+   x
+  =
+  get_c (abstract_rec_rev (S n) p z a b c d e f x).
+Proof.
+intros; simpl; remember (abstract_rec_rev n p z a b c d e f x) as k.
+destruct k as (((((a0,b0),c0),d0),e0),f0); reflexivity.
+Qed.
+
+Lemma abstract_step_rev_d : forall n p (z a b c d e f x : list Z),
+  fd (getbit (Z.of_nat (p - n)) z)
+   (get_a (abstract_rec_rev n p z a b c d e f x))
+   (get_b (abstract_rec_rev n p z a b c d e f x))
+   (get_c (abstract_rec_rev n p z a b c d e f x))
+   (get_d (abstract_rec_rev n p z a b c d e f x))
+   (get_e (abstract_rec_rev n p z a b c d e f x))
+   (get_f (abstract_rec_rev n p z a b c d e f x))
+   x
+  =
+  get_d (abstract_rec_rev (S n) p z a b c d e f x).
+Proof.
+intros; simpl; remember (abstract_rec_rev n p z a b c d e f x) as k.
+destruct k as (((((a0,b0),c0),d0),e0),f0); reflexivity.
+Qed.
+
+Lemma abstract_step_rev_e : forall n p (z a b c d e f x : list Z),
+  fe (getbit (Z.of_nat (p - n)) z)
+   (get_a (abstract_rec_rev n p z a b c d e f x))
+   (get_b (abstract_rec_rev n p z a b c d e f x))
+   (get_c (abstract_rec_rev n p z a b c d e f x))
+   (get_d (abstract_rec_rev n p z a b c d e f x))
+   (get_e (abstract_rec_rev n p z a b c d e f x))
+   (get_f (abstract_rec_rev n p z a b c d e f x))
+   x
+  =
+  get_e (abstract_rec_rev (S n) p z a b c d e f x).
+Proof.
+intros; simpl; remember (abstract_rec_rev n p z a b c d e f x) as k.
+destruct k as (((((a0,b0),c0),d0),e0),f0); reflexivity.
+Qed.
+
+Lemma abstract_step_rev_f : forall n p (z a b c d e f x : list Z),
+  ff (getbit (Z.of_nat (p - n)) z)
+   (get_a (abstract_rec_rev n p z a b c d e f x))
+   (get_b (abstract_rec_rev n p z a b c d e f x))
+   (get_c (abstract_rec_rev n p z a b c d e f x))
+   (get_d (abstract_rec_rev n p z a b c d e f x))
+   (get_e (abstract_rec_rev n p z a b c d e f x))
+   (get_f (abstract_rec_rev n p z a b c d e f x))
+   x
+  =
+  get_f (abstract_rec_rev (S n) p z a b c d e f x).
+Proof.
+intros; simpl; remember (abstract_rec_rev n p z a b c d e f x) as k.
+destruct k as (((((a0,b0),c0),d0),e0),f0); reflexivity.
+Qed.
+
+Close Scope Z.
+
+Variable A_length : forall a b, length a = 16 -> length b = 16 -> length (A a b) = 16.
+Variable M_length : forall a b, length a = 16 -> length b = 16 -> length (M a b) = 16.
+Variable Zub_length : forall a b, length a = 16 -> length b = 16 -> length (Zub a b) = 16.
+Variable Sq_length : forall a, length a = 16 -> length (Sq a) = 16.
+Variable Sel25519_length : forall b p q, length p = 16 -> length q = 16 -> length (Sel25519 b p q) = 16.
+Variable _121665_length : length _121665 = 16.
+
+Open Scope Z.
+
+Variable A_Zlength : forall a b, Zlength a = 16 -> Zlength b = 16 -> Zlength (A a b) = 16.
+Variable M_Zlength : forall a b, Zlength a = 16 -> Zlength b = 16 -> Zlength (M a b) = 16.
+Variable Zub_Zlength : forall a b, Zlength a = 16 -> Zlength b = 16 -> Zlength (Zub a b) = 16.
+Variable Sq_Zlength : forall a, Zlength a = 16 -> Zlength (Sq a) = 16.
+Variable Sel25519_Zlength : forall b p q, Zlength p = 16 -> Zlength q = 16 -> Zlength (Sel25519 b p q) = 16.
+Variable _121665_Zlength : Zlength _121665 = 16.
+
+Close Scope Z.
+
+Local Ltac solve_dependencies_length :=
+  intros;
+  repeat match goal with
+    | _ => omega
+    | _ => apply Sel25519_length
+    | _ => apply M_length
+    | _ => apply Sq_length
+    | _ => apply A_length
+    | _ => apply Zub_length
+    | _ => apply Sel25519_Zlength
+    | _ => apply M_Zlength
+    | _ => apply Sq_Zlength
+    | _ => apply A_Zlength
+    | _ => apply Zub_Zlength
+  end ; reflexivity.
+
+Lemma fa_length : forall r a b c d e f x,
+  length a = 16 -> length b = 16 -> length c = 16 ->
+  length d = 16 -> length e = 16 -> length f = 16 -> length x = 16 ->
+  length (fa r a b c d e f x) = 16.
+Proof. apply (fa_length _ _ _ _ _121665) ; solve_dependencies_length. Qed.
+Lemma fb_length : forall r a b c d e f x,
+  length a = 16 -> length b = 16 -> length c = 16 ->
+  length d = 16 -> length e = 16 -> length f = 16 -> length x = 16 ->
+  length (fb r a b c d e f x) = 16.
+Proof. apply (fb_length _ _ _ _ _121665) ; solve_dependencies_length. Qed.
+Lemma fc_length : forall r a b c d e f x,
+  length a = 16 -> length b = 16 -> length c = 16 ->
+  length d = 16 -> length e = 16 -> length f = 16 -> length x = 16 ->
+  length (fc r a b c d e f x) = 16.
+Proof. apply (fc_length _ _ _ _ _121665) ; solve_dependencies_length. Qed.
+Lemma fd_length : forall r a b c d e f x,
+  length a = 16 -> length b = 16 -> length c = 16 ->
+  length d = 16 -> length e = 16 -> length f = 16 -> length x = 16 ->
+  length (fd r a b c d e f x) = 16.
+Proof. apply (fd_length _ _ _ _ _121665) ; solve_dependencies_length. Qed.
+Lemma fe_length : forall r a b c d e f x,
+  length a = 16 -> length b = 16 -> length c = 16 ->
+  length d = 16 -> length e = 16 -> length f = 16 -> length x = 16 ->
+  length (fe r a b c d e f x) = 16.
+Proof. apply (fe_length _ _ _ _121665) ; solve_dependencies_length. Qed.
+Lemma ff_length : forall r a b c d e f x,
+  length a = 16 -> length b = 16 -> length c = 16 ->
+  length d = 16 -> length e = 16 -> length f = 16 -> length x = 16 ->
+  length (ff r a b c d e f x) = 16.
+Proof. apply (ff_length _ _ _121665) ; solve_dependencies_length. Qed.
+
+Open Scope Z.
+
+Lemma fa_Zlength : forall r a b c d e f x,
+  Zlength a = 16 -> Zlength b = 16 -> Zlength c = 16 ->
+  Zlength d = 16 -> Zlength e = 16 -> Zlength f = 16 -> Zlength x = 16 ->
+  Zlength (fa r a b c d e f x) = 16.
+Proof. apply (fa_Zlength _ _ _ _ _121665) ; solve_dependencies_length. Qed.
+Lemma fb_Zlength : forall r a b c d e f x,
+  Zlength a = 16 -> Zlength b = 16 -> Zlength c = 16 ->
+  Zlength d = 16 -> Zlength e = 16 -> Zlength f = 16 -> Zlength x = 16 ->
+  Zlength (fb r a b c d e f x) = 16.
+Proof. apply (fb_Zlength _ _ _ _ _121665) ; solve_dependencies_length. Qed.
+Lemma fc_Zlength : forall r a b c d e f x,
+  Zlength a = 16 -> Zlength b = 16 -> Zlength c = 16 ->
+  Zlength d = 16 -> Zlength e = 16 -> Zlength f = 16 -> Zlength x = 16 ->
+  Zlength (fc r a b c d e f x) = 16.
+Proof. apply (fc_Zlength _ _ _ _ _121665) ; solve_dependencies_length. Qed.
+Lemma fd_Zlength : forall r a b c d e f x,
+  Zlength a = 16 -> Zlength b = 16 -> Zlength c = 16 ->
+  Zlength d = 16 -> Zlength e = 16 -> Zlength f = 16 -> Zlength x = 16 ->
+  Zlength (fd r a b c d e f x) = 16.
+Proof. apply (fd_Zlength _ _ _ _ _121665) ; solve_dependencies_length. Qed.
+Lemma fe_Zlength : forall r a b c d e f x,
+  Zlength a = 16 -> Zlength b = 16 -> Zlength c = 16 ->
+  Zlength d = 16 -> Zlength e = 16 -> Zlength f = 16 -> Zlength x = 16 ->
+  Zlength (fe r a b c d e f x) = 16.
+Proof. apply (fe_Zlength _ _ _ _121665) ; solve_dependencies_length. Qed.
+Lemma ff_Zlength : forall r a b c d e f x,
+  Zlength a = 16 -> Zlength b = 16 -> Zlength c = 16 ->
+  Zlength d = 16 -> Zlength e = 16 -> Zlength f = 16 -> Zlength x = 16 ->
+  Zlength (ff r a b c d e f x) = 16.
+Proof. apply (ff_Zlength _ _ _121665) ; solve_dependencies_length. Qed.
+
+Close Scope Z.
+
+Lemma abstract_rec_length : forall n p z a b c d e f x a' b' c' d' e' f',
+  length a = 16 -> length b = 16 -> length c = 16 ->
+  length d = 16 -> length e = 16 -> length f = 16 -> length x = 16 ->
+  (a',b',c',d',e',f') = (abstract_rec_rev n p z a b c d e f x) -> 
+  length a' = 16 
+  /\ length b' = 16
+   /\ length c' = 16
+    /\ length d' = 16
+     /\ length e' = 16
+      /\ length f' = 16.
+Proof. induction n ; intros. go.
+simpl in H6.
+remember (abstract_rec_rev n p z a b c d e f x) as k.
+destruct k as (((((a0,b0),c0),d0),e0),f0).
+inversion H6.
+assert(Ht:= IHn p z a b c d e f x a0 b0 c0 d0 e0 f0 H H0 H1 H2 H3 H4 H5 Heqk).
+jauto_set.
+apply fa_length ; auto.
+apply fb_length ; auto.
+apply fc_length ; auto.
+apply fd_length ; auto.
+apply fe_length ; auto.
+apply ff_length ; auto.
+Qed.
+
+Lemma get_a_abstract_rec_length : forall n p z a b c d e f x,
+  length a = 16 -> length b = 16 -> length c = 16 ->
+  length d = 16 -> length e = 16 -> length f = 16 -> length x = 16 ->
+  length (get_a (abstract_rec_rev n p z a b c d e f x)) = 16.
+Proof. intros.
+assert(He: exists a' b' c' d' e' f', (a',b',c',d',e',f') = (abstract_rec_rev n p z a b c d e f x)).
+  remember (abstract_rec_rev n p z a b c d e f x) as k ; destruct k as (((((a0,b0),c0),d0),e0),f0).
+  do 6 eexists ; reflexivity.
+destruct He as [a' [b' [c' [d' [e' [f' He]]]]]].
+assert(Ht := abstract_rec_length n p z a b c d e f x a' b' c' d' e' f' H H0 H1 H2 H3 H4 H5 He).
+rewrite -He; jauto_set; go.
+Qed.
+
+Lemma get_b_abstract_rec_length : forall n p z a b c d e f x,
+  length a = 16 -> length b = 16 -> length c = 16 ->
+  length d = 16 -> length e = 16 -> length f = 16 -> length x = 16 ->
+  length (get_b (abstract_rec_rev n p z a b c d e f x)) = 16.
+Proof. intros.
+assert(He: exists a' b' c' d' e' f', (a',b',c',d',e',f') = (abstract_rec_rev n p z a b c d e f x)).
+  remember (abstract_rec_rev n p z a b c d e f x) as k ; destruct k as (((((a0,b0),c0),d0),e0),f0).
+  do 6 eexists ; reflexivity.
+destruct He as [a' [b' [c' [d' [e' [f' He]]]]]].
+assert(Ht := abstract_rec_length n p z a b c d e f x a' b' c' d' e' f' H H0 H1 H2 H3 H4 H5 He).
+rewrite -He; jauto_set; go.
+Qed.
+
+Lemma get_c_abstract_rec_length : forall n p z a b c d e f x,
+  length a = 16 -> length b = 16 -> length c = 16 ->
+  length d = 16 -> length e = 16 -> length f = 16 -> length x = 16 ->
+  length (get_c (abstract_rec_rev n p z a b c d e f x)) = 16.
+Proof. intros.
+assert(He: exists a' b' c' d' e' f', (a',b',c',d',e',f') = (abstract_rec_rev n p z a b c d e f x)).
+  remember (abstract_rec_rev n p z a b c d e f x) as k ; destruct k as (((((a0,b0),c0),d0),e0),f0).
+  do 6 eexists ; reflexivity.
+destruct He as [a' [b' [c' [d' [e' [f' He]]]]]].
+assert(Ht := abstract_rec_length n p z a b c d e f x a' b' c' d' e' f' H H0 H1 H2 H3 H4 H5 He).
+rewrite -He; jauto_set; go.
+Qed.
+
+Lemma get_d_abstract_rec_length : forall n p z a b c d e f x,
+  length a = 16 -> length b = 16 -> length c = 16 ->
+  length d = 16 -> length e = 16 -> length f = 16 -> length x = 16 ->
+  length (get_d (abstract_rec_rev n p z a b c d e f x)) = 16.
+Proof. intros.
+assert(He: exists a' b' c' d' e' f', (a',b',c',d',e',f') = (abstract_rec_rev n p z a b c d e f x)).
+  remember (abstract_rec_rev n p z a b c d e f x) as k ; destruct k as (((((a0,b0),c0),d0),e0),f0).
+  do 6 eexists ; reflexivity.
+destruct He as [a' [b' [c' [d' [e' [f' He]]]]]].
+assert(Ht := abstract_rec_length n p z a b c d e f x a' b' c' d' e' f' H H0 H1 H2 H3 H4 H5 He).
+rewrite -He; jauto_set; go.
+Qed.
+
+Lemma get_e_abstract_rec_length : forall n p z a b c d e f x,
+  length a = 16 -> length b = 16 -> length c = 16 ->
+  length d = 16 -> length e = 16 -> length f = 16 -> length x = 16 ->
+  length (get_e (abstract_rec_rev n p z a b c d e f x)) = 16.
+Proof. intros.
+assert(He: exists a' b' c' d' e' f', (a',b',c',d',e',f') = (abstract_rec_rev n p z a b c d e f x)).
+  remember (abstract_rec_rev n p z a b c d e f x) as k ; destruct k as (((((a0,b0),c0),d0),e0),f0).
+  do 6 eexists ; reflexivity.
+destruct He as [a' [b' [c' [d' [e' [f' He]]]]]].
+assert(Ht := abstract_rec_length n p z a b c d e f x a' b' c' d' e' f' H H0 H1 H2 H3 H4 H5 He).
+rewrite -He; jauto_set; go.
+Qed.
+
+Lemma get_f_abstract_rec_length : forall n p z a b c d e f x,
+  length a = 16 -> length b = 16 -> length c = 16 ->
+  length d = 16 -> length e = 16 -> length f = 16 -> length x = 16 ->
+  length (get_f (abstract_rec_rev n p z a b c d e f x)) = 16.
+Proof. intros.
+assert(He: exists a' b' c' d' e' f', (a',b',c',d',e',f') = (abstract_rec_rev n p z a b c d e f x)).
+  remember (abstract_rec_rev n p z a b c d e f x) as k ; destruct k as (((((a0,b0),c0),d0),e0),f0).
+  do 6 eexists ; reflexivity.
+destruct He as [a' [b' [c' [d' [e' [f' He]]]]]].
+assert(Ht := abstract_rec_length n p z a b c d e f x a' b' c' d' e' f' H H0 H1 H2 H3 H4 H5 He).
+rewrite -He; jauto_set; go.
+Qed.
+
+Open Scope Z.
+
+Lemma abstract_rec_Zlength : forall n p z a b c d e f x a' b' c' d' e' f',
+  Zlength a = 16 -> Zlength b = 16 -> Zlength c = 16 ->
+  Zlength d = 16 -> Zlength e = 16 -> Zlength f = 16 -> Zlength x = 16 ->
+  (a',b',c',d',e',f') = (abstract_rec_rev n p z a b c d e f x) -> 
+  Zlength a' = 16 
+  /\ Zlength b' = 16
+   /\ Zlength c' = 16
+    /\ Zlength d' = 16
+     /\ Zlength e' = 16
+      /\ Zlength f' = 16.
+Proof. induction n ; intros. go.
+simpl in H6.
+remember (abstract_rec_rev n p z a b c d e f x) as k.
+destruct k as (((((a0,b0),c0),d0),e0),f0).
+inversion H6.
+assert(Ht:= IHn p z a b c d e f x a0 b0 c0 d0 e0 f0 H H0 H1 H2 H3 H4 H5 Heqk).
+jauto_set.
+apply fa_Zlength ; auto.
+apply fb_Zlength ; auto.
+apply fc_Zlength ; auto.
+apply fd_Zlength ; auto.
+apply fe_Zlength ; auto.
+apply ff_Zlength ; auto.
+Qed.
+
+Lemma get_a_abstract_rec_Zlength : forall n p z a b c d e f x,
+  Zlength a = 16 -> Zlength b = 16 -> Zlength c = 16 ->
+  Zlength d = 16 -> Zlength e = 16 -> Zlength f = 16 -> Zlength x = 16 ->
+  Zlength (get_a (abstract_rec_rev n p z a b c d e f x)) = 16.
+Proof. intros.
+assert(He: exists a' b' c' d' e' f', (a',b',c',d',e',f') = (abstract_rec_rev n p z a b c d e f x)).
+  remember (abstract_rec_rev n p z a b c d e f x) as k ; destruct k as (((((a0,b0),c0),d0),e0),f0).
+  do 6 eexists ; reflexivity.
+destruct He as [a' [b' [c' [d' [e' [f' He]]]]]].
+assert(Ht := abstract_rec_Zlength n p z a b c d e f x a' b' c' d' e' f' H H0 H1 H2 H3 H4 H5 He).
+rewrite -He; jauto_set; go.
+Qed.
+
+Lemma get_b_abstract_rec_Zlength : forall n p z a b c d e f x,
+  Zlength a = 16 -> Zlength b = 16 -> Zlength c = 16 ->
+  Zlength d = 16 -> Zlength e = 16 -> Zlength f = 16 -> Zlength x = 16 ->
+  Zlength (get_b (abstract_rec_rev n p z a b c d e f x)) = 16.
+Proof. intros.
+assert(He: exists a' b' c' d' e' f', (a',b',c',d',e',f') = (abstract_rec_rev n p z a b c d e f x)).
+  remember (abstract_rec_rev n p z a b c d e f x) as k ; destruct k as (((((a0,b0),c0),d0),e0),f0).
+  do 6 eexists ; reflexivity.
+destruct He as [a' [b' [c' [d' [e' [f' He]]]]]].
+assert(Ht := abstract_rec_Zlength n p z a b c d e f x a' b' c' d' e' f' H H0 H1 H2 H3 H4 H5 He).
+rewrite -He; jauto_set; go.
+Qed.
+
+Lemma get_c_abstract_rec_Zlength : forall n p z a b c d e f x,
+  Zlength a = 16 -> Zlength b = 16 -> Zlength c = 16 ->
+  Zlength d = 16 -> Zlength e = 16 -> Zlength f = 16 -> Zlength x = 16 ->
+  Zlength (get_c (abstract_rec_rev n p z a b c d e f x)) = 16.
+Proof. intros.
+assert(He: exists a' b' c' d' e' f', (a',b',c',d',e',f') = (abstract_rec_rev n p z a b c d e f x)).
+  remember (abstract_rec_rev n p z a b c d e f x) as k ; destruct k as (((((a0,b0),c0),d0),e0),f0).
+  do 6 eexists ; reflexivity.
+destruct He as [a' [b' [c' [d' [e' [f' He]]]]]].
+assert(Ht := abstract_rec_Zlength n p z a b c d e f x a' b' c' d' e' f' H H0 H1 H2 H3 H4 H5 He).
+rewrite -He; jauto_set; go.
+Qed.
+
+Lemma get_d_abstract_rec_Zlength : forall n p z a b c d e f x,
+  Zlength a = 16 -> Zlength b = 16 -> Zlength c = 16 ->
+  Zlength d = 16 -> Zlength e = 16 -> Zlength f = 16 -> Zlength x = 16 ->
+  Zlength (get_d (abstract_rec_rev n p z a b c d e f x)) = 16.
+Proof. intros.
+assert(He: exists a' b' c' d' e' f', (a',b',c',d',e',f') = (abstract_rec_rev n p z a b c d e f x)).
+  remember (abstract_rec_rev n p z a b c d e f x) as k ; destruct k as (((((a0,b0),c0),d0),e0),f0).
+  do 6 eexists ; reflexivity.
+destruct He as [a' [b' [c' [d' [e' [f' He]]]]]].
+assert(Ht := abstract_rec_Zlength n p z a b c d e f x a' b' c' d' e' f' H H0 H1 H2 H3 H4 H5 He).
+rewrite -He; jauto_set; go.
+Qed.
+
+Lemma get_e_abstract_rec_Zlength : forall n p z a b c d e f x,
+  Zlength a = 16 -> Zlength b = 16 -> Zlength c = 16 ->
+  Zlength d = 16 -> Zlength e = 16 -> Zlength f = 16 -> Zlength x = 16 ->
+  Zlength (get_e (abstract_rec_rev n p z a b c d e f x)) = 16.
+Proof. intros.
+assert(He: exists a' b' c' d' e' f', (a',b',c',d',e',f') = (abstract_rec_rev n p z a b c d e f x)).
+  remember (abstract_rec_rev n p z a b c d e f x) as k ; destruct k as (((((a0,b0),c0),d0),e0),f0).
+  do 6 eexists ; reflexivity.
+destruct He as [a' [b' [c' [d' [e' [f' He]]]]]].
+assert(Ht := abstract_rec_Zlength n p z a b c d e f x a' b' c' d' e' f' H H0 H1 H2 H3 H4 H5 He).
+rewrite -He; jauto_set; go.
+Qed.
+
+Lemma get_f_abstract_rec_Zlength : forall n p z a b c d e f x,
+  Zlength a = 16 -> Zlength b = 16 -> Zlength c = 16 ->
+  Zlength d = 16 -> Zlength e = 16 -> Zlength f = 16 -> Zlength x = 16 ->
+  Zlength (get_f (abstract_rec_rev n p z a b c d e f x)) = 16.
+Proof. intros.
+assert(He: exists a' b' c' d' e' f', (a',b',c',d',e',f') = (abstract_rec_rev n p z a b c d e f x)).
+  remember (abstract_rec_rev n p z a b c d e f x) as k ; destruct k as (((((a0,b0),c0),d0),e0),f0).
+  do 6 eexists ; reflexivity.
+destruct He as [a' [b' [c' [d' [e' [f' He]]]]]].
+assert(Ht := abstract_rec_Zlength n p z a b c d e f x a' b' c' d' e' f' H H0 H1 H2 H3 H4 H5 He).
+rewrite -He; jauto_set; go.
+Qed.
+
+Close Scope Z.
+
+End ScalarRec.
